new/proof/github_com/goose_lang/goose/model/channel/chan_spec_select.v
@@ -1,8 +1,11 @@
 From New.proof.github_com.goose_lang Require Import primitive.
 From New.proof.github_com.goose_lang.std Require Import std_core.
-From New.proof.github_com.goose_lang.goose.model.channel Require Import chan_ghost_state chan_spec_inv chan_spec_base.
+From New.proof.github_com.goose_lang.goose.model.channel Require Import chan_ghost_state chan_spec_inv chan_spec_base chan_spec_send chan_spec_recv.
 From New.generatedproof.github_com.goose_lang.goose Require Import model.channel.
 From New.proof Require Import proof_prelude.
+Require Export New.code.sync.
+Require Export New.generatedproof.sync.
+From New.proof.sync_proof Require Import base mutex sema.
 
 Section proof.
 Context `{hG: heapGS Σ, !ffi_semantics _ _}. 
@@ -28,13 +31,15 @@ match selected with
     end
 end.
 
-Definition nil_select_case : loc := null.
-
 Definition own_select_case
   (dir: select_dir) (params: chan) (case_ptr: loc) (selected: bool) (i: nat) (v': val) : iProp Σ :=
-  if bool_decide (case_ptr = nil_select_case) then
+  if bool_decide (params.(ch_loc) = null) then
     (* For nil case, precondition is True, postcondition is False *)
-    (if selected then False%I else True%I)%I
+    (if selected then False%I else 
+      "%Hintty" ∷ ⌜params.(ch_T) = int64T⌝ ∗  (* This connects v' to a properly typed v *)
+      "chan_ptr" ∷ case_ptr ↦s[(channel.SelectCase.ty params.(ch_T)) :: "channel"] null
+    
+    %I)%I
   else
     (let T' := params.(ch_T') in
     let T := params.(ch_T) in
@@ -42,210 +47,281 @@ Definition own_select_case
     let IntoValTyped_inst := params.(ch_IntoValTyped) in
     let Hbounded := params.(ch_Hbounded) in
     ∃  (v: T') (ok: bool),
-      "%Hvalconv" ∷ ⌜v' = to_val v⌝ ∗  (* This connects v' to a properly typed v *)
-      "channel" ∷ case_ptr ↦s[(channel.SelectCase.ty T) :: "channel"] params.(ch_loc) ∗
+      (*"%Hvalconv" ∷ ⌜v' = to_val v⌝ ∗  (* This connects v' to a properly typed v *) *)
+      "chan_ptr" ∷ case_ptr ↦s[(channel.SelectCase.ty T) :: "channel"] params.(ch_loc) ∗
       "dir" ∷ case_ptr ↦s[(channel.SelectCase.ty T) :: "dir"] (select_dir_to_word dir) ∗
       "Value" ∷ case_ptr ↦s[(channel.SelectCase.ty T) :: "Value"] v ∗
       "Ok" ∷ case_ptr ↦s[(channel.SelectCase.ty T) :: "Ok"] ok ∗ 
       "Hlogicalselect" ∷ own_select_case_logical params dir v selected i ok)%I.
 
-Definition own_selected_case_multi
-  (blocking: bool) (selected_index: nat)
-  (params1 params2 params3 params4 params5: chan)
-  (dir1 dir2 dir3 dir4 dir5: select_dir) 
-  (case1 case2 case3 case4 case5: loc) 
-  (v1 v2 v3 v4 v5: val) 
-  (i1 i2 i3 i4 i5: nat) : iProp Σ :=
-  let cases := [case1; case2; case3; case4; case5] in
-  if (bool_decide (selected_index < 5)) then
-    ("%Hindlt5" ∷ ⌜selected_index < 5⌝ ∗
-     ("Hselcase" ∷ match selected_index with
-     | 0%nat => own_select_case dir1 params1 case1 true i1 v1
-     | 1%nat => own_select_case dir2 params2 case2 true i2 v2
-     | 2%nat => own_select_case dir3 params3 case3 true i3 v3
-     | 3%nat => own_select_case dir4 params4 case4 true i4 v4
-     | 4%nat => own_select_case dir5 params5 case5 true i5 v5
-     | _ => False
-     end)%I ∗
-     ("Hcase1" ∷ (if decide(selected_index ≠ 0%nat) then  own_select_case dir1 params1 case1 false i1 v1 else True)) ∗
-     ("Hcase2" ∷ (if decide(selected_index ≠ 1%nat) then  own_select_case dir2 params2 case2 false i2 v2 else True)) ∗
-     ("Hcase3" ∷ (if decide(selected_index ≠ 2%nat) then  own_select_case dir3 params3 case3 false i3 v3 else True)) ∗
-     ("Hcase4" ∷ (if decide(selected_index ≠ 3%nat) then  own_select_case dir4 params4 case4 false i4 v4 else True)) ∗
-     ("Hcase5" ∷ (if decide(selected_index ≠ 4%nat) then  own_select_case dir5 params5 case5 false i5 v5 else True)) )%I
-  else
-    ⌜selected_index = 5%nat ∧ ¬ blocking⌝%I.
 
-Definition own_selected_case_params1
-  (dir1: select_dir) (params1: chan) (blocking: bool) (selected_index: nat) 
-  (case1: loc) (v1: val) (i1: nat) : iProp Σ :=
-  own_selected_case_multi blocking selected_index 
-    params1 params1 params1 params1 params1
-    dir1 dir1 dir1 dir1 dir1
-    case1 nil_select_case nil_select_case nil_select_case nil_select_case
-    v1 v1 v1 v1 v1
-    i1 i1 i1 i1 i1.
+Lemma wp_TrySelect (params: chan) (dir: select_dir) (case_ptr: loc) 
+      (i: nat) (v: params.(ch_T')):
+      let IntoVal_inst := params.(ch_IntoVal) in
+      let IntoValTyped_inst := params.(ch_IntoValTyped) in
+      {{{ is_pkg_init channel ∗ own_select_case dir params case_ptr false i #v }}}
+        channel @ "TrySelect" #params.(ch_T) #case_ptr
+      {{{ (selected: bool), RET #selected;
+          own_select_case dir params case_ptr selected i #v
+      }}}.
+    Proof.
+      intros Hiv_inst Hivt_inst.
+      wp_start. wp_auto.
+      unfold own_select_case.
+      destruct bool_decide eqn:Hb.
+      {
+        iNamed "Hpre".  replace params.(ch_T) with int64T.
+        wp_auto. 
+        iApply "HΦ". iFrame. done.
+      }
+      {
+        iNamed "Hpre".
+        wp_auto. rewrite Hb. wp_auto. wp_if_destruct.
+        {
+         wp_auto.
+         Search wp_Channel__TrySend.
+         unfold own_select_case_logical.
+          assert (dir = SelectSend).
+         {
+          destruct dir;first done;done.
+         }
+         subst dir.
+         iNamed "Hlogicalselect".
+         iNamed "HCh".
+         wp_apply (wp_Channel__TrySend params i v0 with "[HSc  HP  ]"). all: try done;try lia; try word.
+         {
+          iFrame "#". iFrame. iPureIntro. done.
+         }
+         {
+          iIntros (selected) "Hsel".
+          
+          wp_auto. iApply "HΦ".
+          destruct selected.
+          {
+           iFrame. 
+          }
+          {
+           iFrame.  
+          }
+         }
+        }
+        {
+         wp_auto. wp_if_destruct.
+         {
+          wp_auto.
+          assert (dir = SelectRecv).
+         {
+          destruct dir;first done;done.
+         }
+          iNamed "Hlogicalselect".
+          unfold own_select_case_logical. subst dir.
+          iNamed "Hlogicalselect".
+          wp_apply (wp_Channel__TryReceive params i with "[HCh HQ HRecvPerm]").
+          all: try done.
+          {
+           iFrame. done. 
+          }
+          iIntros (v1).
+          iIntros (ok1).
+          iIntros (selected).
+          destruct selected.
+          {
+            iIntros "Hrecvpost".
+           wp_auto. iApply "HΦ". iFrame.  
+          }
+          {
+            iIntros "HRecvpre".
+           wp_auto. iApply "HΦ". iFrame.  
+          }
+         }
+         {
+          iApply "HΦ". iFrame.
+         }
+        }
+      }
+    Qed.
 
-
-Definition own_selected_case_params2
-  (dir1 dir2: select_dir) (params1 params2: chan) (blocking: bool) (selected_index: nat) 
-  (case1 case2: loc) (v1 v2: val) (i1 i2: nat) : iProp Σ :=
-  own_selected_case_multi blocking selected_index 
-    params1 params2 params1 params1 params1
-    dir1 dir2 dir1 dir1 dir1
-    case1 case2 nil_select_case nil_select_case nil_select_case
-    v1 v2 v1 v1 v1
-    i1 i2 i1 i1 i1.
-
-Definition own_selected_case_params3
-    (dir1 dir2 dir3: select_dir)
-    (params1 params2 params3: chan)
-    (blocking: bool) (selected_index: nat)
-    (case1 case2 case3: loc)
-    (v1 v2 v3: val) (i1 i2 i3: nat) : iProp Σ :=
-    own_selected_case_multi blocking selected_index 
-      params1 params2 params3 params1 params1
-      dir1 dir2 dir3 dir1 dir1
-      case1 case2 case3 nil_select_case nil_select_case
-      v1 v2 v3 v1 v1
-      i1 i2 i3 i1 i1.
-  
-Definition own_selected_case_params4
-  (dir1 dir2 dir3 dir4: select_dir)
-  (params1 params2 params3 params4: chan)
-  (blocking: bool) (selected_index: nat)
-  (case1 case2 case3 case4: loc)
-  (v1 v2 v3 v4: val) (i1 i2 i3 i4: nat) : iProp Σ :=
-  own_selected_case_multi blocking selected_index 
-    params1 params2 params3 params4 params1
-    dir1 dir2 dir3 dir4 dir1
-    case1 case2 case3 case4 nil_select_case
-    v1 v2 v3 v4 v1
-    i1 i2 i3 i4 i1.
-
-Definition own_selected_case_params5
-  (dir1 dir2 dir3 dir4 dir5: select_dir)
-  (params1 params2 params3 params4 params5: chan)
-  (blocking: bool) (selected_index: nat)
-  (case1 case2 case3 case4 case5: loc)
-  (v1 v2 v3 v4 v5: val) (i1 i2 i3 i4 i5: nat) : iProp Σ :=
-  own_selected_case_multi blocking selected_index 
-    params1 params2 params3 params4 params5
-    dir1 dir2 dir3 dir4 dir5
-    case1 case2 case3 case4 case5
-    v1 v2 v3 v4 v5
-    i1 i2 i3 i4 i5.
-
-Lemma wp_multiSelect
-    (params1 params2 params3 params4 params5: chan)
-    (dir1 dir2 dir3 dir4 dir5: select_dir) 
-    (case1 case2 case3 case4 case5 : loc)
-    (v1 v2 v3 v4 v5: val)
-    (i1 i2 i3 i4 i5: nat)
+    Lemma wp_Select1
+    (params1: chan)
+    (dir1: select_dir)
+    (case1 : loc)
+    (i1: nat) (v1: params1.(ch_T'))
     (blocking : bool) :
-  {{{
-      is_pkg_init channel ∗ 
-  own_select_case dir1 params1 case1 false i1 v1 ∗
-      own_select_case dir2 params2 case2 false i2 v2 ∗
-      own_select_case dir3 params3 case3 false i3 v3 ∗
-      own_select_case dir4 params4 case4 false i4 v4 ∗
-      own_select_case dir5 params5 case5 false i5 v5 }}}
-    channel @ "multiSelect" #params1.(ch_T) #params2.(ch_T) #params3.(ch_T) #params4.(ch_T) #params5.(ch_T)  #case1 #case2 #case3 #case4 #case5 #blocking
-  {{{ (selected_index : nat), RET #(W64 selected_index); 
-      own_selected_case_params5 dir1 dir2 dir3 dir4 dir5 params1 params2 params3 params4 params5
-       blocking selected_index 
-                               case1 case2 case3 case4 case5 v1 v2 v3 v4 v5 i1 i2 i3 i4 i5 }}}.
-  Proof.
-  wp_start. wp_auto. 
-  Admitted.
-
-Lemma wp_TrySelectAt
-  (params: chan)
-  (dir: select_dir)
-  (case_ptr : loc)
-  (i: nat) (v: val)
-  :
-  {{{ is_pkg_init channel ∗  own_select_case dir params case_ptr false i v }}}
-    channel @ "TrySelectAt" #params.(ch_T) #case_ptr
-  {{{ (selected : bool), RET #selected;
-      own_select_case dir params case_ptr selected i v }}}.
-Proof.
-  wp_start. wp_auto.
-Admitted.
-
-Definition is_perm_0_5 (order : list nat) : Prop :=
-  Permutation order [0%nat;1%nat;2%nat;3%nat;4%nat].
-
-Definition nats_to_u64s (ns : list nat) : list u64 :=
-  List.map (λ n, W64 (Z.of_nat n)) ns.
-
-Definition own_order_slice (s: slice.t) (order: list nat) : iProp Σ :=
-  ⌜is_perm_0_5 order⌝ ∗
-  own_slice s (DfracOwn 1) (nats_to_u64s order).
-
-(* Helper function to select the right params, index, and value based on index *)
-Definition select_case_info_by_index 
-  (idx: nat) 
-  (params1 params2 params3 params4 params5: @chan _ Σ)
-  (dir1 dir2 dir3 dir4 dir5: select_dir) 
-  (i1 i2 i3 i4 i5: nat)
-  (v1 v2 v3 v4 v5: val) : 
-  (chan * select_dir * nat * val) :=
-  match idx with
-  | 0%nat => (params1, dir1, i1, v1)
-  | 1%nat => (params2, dir2, i2, v2)
-  | 2%nat => (params3, dir3, i3, v3)
-  | 3%nat => (params4, dir4, i4, v4)
-  | _ => (params5, dir5, i5, v5)
-  end.
-
-Lemma wp_TrySelectCase
-  (params1 params2 params3 params4 params5: chan)
-  (dir1 dir2 dir3 dir4 dir5: select_dir) 
-  (i1 i2 i3 i4 i5: nat)
-  (v1 v2 v3 v4 v5: val)
-  (idx : nat) (case1 case2 case3 case4 case5 : loc):
-  0 ≤ idx < 5 →
-  let '(params_i, dir_i, i, v) := select_case_info_by_index idx params1 params2 params3 params4 params5 dir1 dir2 dir3 dir4 dir5 i1 i2 i3 i4 i5 v1 v2 v3 v4 v5 in
-  {{{ is_pkg_init channel ∗  own_select_case dir_i params_i (List.nth idx [case1; case2; case3; case4; case5] case1) false i v }}}
-    channel @ "TrySelectCase"  #params1.(ch_T) #params2.(ch_T) #params3.(ch_T) #params4.(ch_T) #params5.(ch_T)  #(W64 idx) #case1 #case2 #case3 #case4 #case5
-  {{{ (selected : bool), RET #selected;
-      own_select_case dir_i params_i (List.nth idx [case1; case2; case3; case4; case5] case1) selected i v }}}.
-Proof.
-  intros Hind.
-    unfold select_case_info_by_index.
-  destruct idx.
-  {
+    let IntoVal_inst1 := params1.(ch_IntoVal) in
+    let IntoValTyped_inst1 := params1.(ch_IntoValTyped) in
+    params1.(ch_loc) ≠ null ->
+    {{{ is_pkg_init channel ∗ own_select_case dir1 params1 case1 false i1 #v1 }}}
+      channel @ "Select1" #params1.(ch_T) #case1 #blocking
+    {{{ (selected : bool), RET #selected;
+       "Hb" ∷ ⌜if blocking then selected else true⌝%I ∗ 
+       if selected then 
+       own_select_case dir1 params1 case1 true i1 #v1 
+        else 
+        own_select_case dir1 params1 case1 false i1 #v1 
+        }}}.
+  Proof. 
+    intros Hiv Hivt Hnn.
     wp_start. wp_auto.
-Admitted.
-      
-Lemma wp_TryCasesInOrder
-  (params1 params2 params3 params4 params5: chan)
-  (dir1 dir2 dir3 dir4 dir5: select_dir) 
-  (i1 i2 i3 i4 i5: nat)
-  (v1 v2 v3 v4 v5: val)
-  (case1 case2 case3 case4 case5 : loc)
-  (order : slice.t)
-  (order_rep : list nat) :
-{{{ 
-  is_pkg_init channel ∗ 
-  own_order_slice order order_rep ∗
-  [∗ list] j ∈ order_rep, 
-    let '(params_j, dir_j, i_j, v_j) := select_case_info_by_index j params1 params2 params3 params4 params5 dir1 dir2 dir3 dir4 dir5 i1 i2 i3 i4 i5 v1 v2 v3 v4 v5 in
-    own_select_case dir_j params_j (List.nth j [case1; case2; case3; case4; case5] case1) false i_j v_j
-}}}
-  channel @ "TryCasesInOrder"  #params1.(ch_T) #params2.(ch_T) #params3.(ch_T) #params4.(ch_T) #params5.(ch_T)
-    #order #case1 #case2 #case3 #case4 #case5
-{{{ (selected_idx : nat), RET #(W64 selected_idx);
-    ⌜selected_idx ≤ 5⌝ ∗
-    ([∗ list] j↦_ ∈ order_rep,
-     let '(params_j, dir_j, i_j, v_j) := select_case_info_by_index j params1 params2 params3 params4 params5 dir1 dir2 dir3 dir4 dir5 i1 i2 i3 i4 i5 v1 v2 v3 v4 v5 in
-     if j =? selected_idx then
-       own_select_case dir_j params_j (List.nth j [case1; case2; case3; case4; case5] case1) true i_j v_j
-     else
-       own_select_case dir_j params_j (List.nth j [case1; case2; case3; case4; case5] case1) false i_j v_j)
-}}}.
+    wp_for. unfold own_select_case. iNamed "Hpre".
+    destruct bool_decide eqn: Hb.
+    {
+      apply bool_decide_eq_true in Hb.
+     done. 
+    }
+    iNamed "Hpre".
+     wp_apply (wp_TrySelect with "[chan_ptr dir Value Ok Hlogicalselect]").
+     {
+      unfold own_select_case.
+      destruct bool_decide.
+      {
+       done. 
+      }
+        iFrame.
+     }
+     iIntros (selected) "Hsel".
+     wp_auto.
+     destruct selected.
+     {
+      wp_auto.
+      wp_for_post. iApply "HΦ". unfold own_select_case.
+      destruct bool_decide.
+      {
+        done.
+      }
+      iFrame. iPureIntro. destruct blocking. all: done.
+     }
+     wp_auto. destruct blocking.
+     {
+      wp_auto. wp_for_post. iFrame. unfold own_select_case.
+      destruct bool_decide.
+      {
+        done.
+      }
+      iFrame.
+     }
+     wp_auto. wp_for_post. iApply "HΦ". unfold own_select_case.
+     destruct bool_decide; first done.
+     iFrame.
+     Unshelve.
+     {
+      iPureIntro. done.
+     }
+     done.
+  Qed.
+
+    Lemma wp_TrySelectCase2 
+    (params1 params2: chan) 
+    (dir1 dir2: select_dir)
+    (case1_ptr case2_ptr: loc)
+    (i1 i2: nat) 
+    (v1: params1.(ch_T')) (v2: params2.(ch_T'))
+    (index: u64):
+    let IntoVal_inst1 := params1.(ch_IntoVal) in
+    let IntoValTyped_inst1 := params1.(ch_IntoValTyped) in
+    let IntoVal_inst2 := params2.(ch_IntoVal) in
+    let IntoValTyped_inst2 := params2.(ch_IntoValTyped) in
+    (index = W64 0 ∨ index = W64 1) ->
+    {{{ is_pkg_init channel ∗
+       "Hc1pre" ∷ own_select_case dir1 params1 case1_ptr false i1 #v1 ∗
+       "Hc2pre" ∷ own_select_case dir2 params2 case2_ptr false i2 #v2
+    }}}
+      channel @ "TrySelectCase2" #params1.(ch_T) #params2.(ch_T) #index #case1_ptr #case2_ptr
+    {{{ (selected: bool), RET #selected;
+        if decide (index = W64 0) then
+          own_select_case dir1 params1 case1_ptr selected i1 #v1 ∗
+          own_select_case dir2 params2 case2_ptr false i2 #v2
+        else (* index = W64 1 *)
+          own_select_case dir1 params1 case1_ptr false i1 #v1 ∗
+          own_select_case dir2 params2 case2_ptr selected i2 #v2
+    }}}.
+  Proof.
+    intros Hiv1 Hivt1 Hiv2 Hivt2 Hindex.
+    wp_start. wp_apply wp_alloc.
+    iNamed "Hpre". 
+    iIntros (case_2) "Hc2p".
+     wp_auto.
+     wp_apply wp_alloc.
+    iIntros (case_1) "Hc1p".
+    wp_auto. 
+    wp_if_destruct.
+    {
+     wp_auto.
+
+     wp_apply (wp_TrySelect params1 dir1 case1_ptr i1 v1 with "[Hc1pre Hc1p]").
+     {
+      iFrame.
+     }
+     iIntros (selected) "Hsc".
+     wp_auto. iApply "HΦ". iFrame.
+    }
+    {
+    wp_auto.
+     wp_if_destruct.
+     {
+      wp_auto. 
+     wp_apply (wp_TrySelect params2 dir2 case2_ptr i2 v2 with "[Hc2pre Hc2p]").
+     {
+      iFrame.
+     }
+     iIntros (selected) "Hsc".
+     wp_auto. iApply "HΦ". iFrame.
+     }
+     word.
+    }
+  Qed.
+
+  Lemma wp_NewSendCase
+  (params: chan) (i: nat) (v: params.(ch_T')):
+  let T' := params.(ch_T') in
+  let T := params.(ch_T) in
+  let IntoVal_inst := params.(ch_IntoVal) in
+  let IntoValTyped_inst := params.(ch_IntoValTyped) in
+  let Hbounded := params.(ch_Hbounded) in
+  {{{ is_pkg_init channel ∗ send_pre params i v }}}
+    channel @ "NewSendCase" #T #params.(ch_loc) #v
+  {{{ (case_ptr: loc), RET #case_ptr;
+      own_select_case SelectSend params case_ptr false i #v
+  }}}.
 Proof.
-  wp_start. wp_auto.
-Admitted.
+  intros HT' HT Hiv_inst Hivt_inst Hb_inst. wp_start. wp_auto. iNamed "Hpre".
+  wp_apply wp_alloc. iIntros (ptr) "Hptr".
+  iApply struct_fields_split in "Hptr"; iNamed "Hptr". wp_auto. iApply "HΦ".
+  iNamed "HCh".
+  unfold own_select_case. simpl.
+  destruct bool_decide eqn: Hb.
+  {
+    apply bool_decide_eq_true in Hb.
+    done.
+  }
+  iFrame.
+  simpl. iFrame "#". iFrame. iPureIntro. done. 
+Qed.
+
+Lemma wp_NewRecvCase
+  (params: chan) (i: nat):
+  let T' := params.(ch_T') in
+  let T := params.(ch_T) in
+  let IntoVal_inst := params.(ch_IntoVal) in
+  let IntoValTyped_inst := params.(ch_IntoValTyped) in
+  let Hbounded := params.(ch_Hbounded) in
+  {{{ is_pkg_init channel ∗ recv_pre params i }}}
+    channel @ "NewRecvCase" #T #params.(ch_loc)
+  {{{ (case_ptr: loc), RET #case_ptr;
+      own_select_case SelectRecv params case_ptr false i (#(default_val params.(ch_T')))
+  }}}.
+Proof.
+  intros H1 H2 Hiv_inst Hivt_inst Hb_inst. wp_start. wp_auto. iNamed "Hpre".
+  wp_apply wp_alloc. iIntros (ptr) "Hptr".
+  iApply struct_fields_split in "Hptr"; iNamed "Hptr". wp_auto. iApply "HΦ".
+  iNamed "HCh".
+  unfold own_select_case. simpl.
+  destruct bool_decide eqn: Hb.
+  {
+    apply bool_decide_eq_true in Hb.
+    done.
+  }
+  iFrame.
+  simpl. iFrame "#". iPureIntro. done.
+Qed.
 
 End proof.
